WIP

RealWorld.v
@@ -50,7 +50,7 @@ Inductive message :=
 | Ciphertext (sender_id : user_id) (msg : message) (k_id : nat)
 | Signature (k_id : nat) (signer_id : user_id) (msg : message)
 | HMAC_Message (sender_id : user_id) (k_id : nat) (msg : message).
-
+ 
 (* Maybe: 
  * Return' (k : key)
  * Return'' (p : (key * key))
@@ -61,492 +61,459 @@ Inductive message :=
    Note: Semantically, GenerateSymKey and GenerateAsymKeys need to return key and key*key, respectively.
          We will define two additional commands ReturnK (k: key) and ReturnKP (p: key * key) to handle this.
          This will allow us to remove the key_pair_message constructor above *)
-Inductive user_cmd :=
-| Return (r : message)
-| Bind (c1 : user_cmd) (c2 : message -> user_cmd)
-| BindSymKey (c1 : user_cmd) (c2 : var -> user_cmd)
-| BindAsymKeys (c1 : user_cmd) (c2 : (var * var) -> user_cmd)
+(* Inductive user_cmd := *)
+(* | Return (r : message) *)
+(* | Bind (c1 : user_cmd) (c2 : message -> user_cmd) *)
+(* | BindSymKey (c1 : user_cmd) (c2 : var -> user_cmd) *)
+(* | BindAsymKeys (c1 : user_cmd) (c2 : (var * var) -> user_cmd) *)
 
-| Send (uid : user_id) (msg : message)
-| Recv
-| Decrypt (k : option var) (ctxt : message)
-| Encrypt (k : var) (ptxt : message)
-| Sign (k : var) (msg : message)
-| Verify (k : option var) (sig : message)
-| ProduceHMAC (k : var) (msg : message)
-| VerifyHMAC (k : option var) (mac : message)
-| GenerateSymKey (usage : symmetric_usage)
-| GenerateAsymKeys (usage : asymmetric_usage)
-| Barrier.
+(* | Send (uid : user_id) (msg : message) *)
+(* | Recv *)
+(* | Decrypt (k : option var) (ctxt : message) *)
+(* | Encrypt (k : var) (ptxt : message) *)
+(* | Sign (k : var) (msg : message) *)
+(* | Verify (k : option var) (sig : message) *)
+(* | ProduceHMAC (k : var) (msg : message) *)
+(* | VerifyHMAC (k : option var) (mac : message) *)
+(* | GenerateSymKey (usage : symmetric_usage) *)
+(* | GenerateAsymKeys (usage : asymmetric_usage) *)
+(* | Barrier. *)
+
+(* Notation "x <- c1 ; c2" := (Bind c1 (fun x => c2)) (right associativity, at level 75). *)
+(* Notation "x <<- c1 ; c2" := (BindSymKey c1 (fun x => c2)) (right associativity, at level 75). *)
+(* Notation "x <<<- c1 ; c2" := (BindAsymKeys c1 (fun x => c2)) (right associativity, at level 75). *)
+
+Inductive user_cmd : Set -> Type :=
+  (* Plumbing *)
+| Return {result : Set} (r : result) : user_cmd result
+| Bind {result result' : Set} (c1 : user_cmd result') (c2 : result' -> user_cmd result) : user_cmd result
+
+| Send (uid : user_id) (msg : message) : user_cmd unit
+| Recv : user_cmd message
+
+| Decrypt (k : var) (ctxt : message) : user_cmd message (* can message be Ciphertext somehow?? *)
+| Encrypt (k : var) (ptxt : message) : user_cmd message
+
+| Sign (k : var) (msg : message) : user_cmd message
+| Verify (k : option var) (sig : message) : user_cmd message
+
+| ProduceHMAC (k : var) (msg : message) : user_cmd message
+| VerifyHMAC (k : option var) (mac : message) : user_cmd message
+
+| GenerateSymKey (usage : symmetric_usage) : user_cmd var
+| GenerateAsymKeys (usage : asymmetric_usage) : user_cmd (var * var)
+
+(* Allow administrator to make some global change to the universe -- revoke keys, etc. *)
+(* This may be a universe level step -- Administrator forces all users to stop *)
+| Barrier {result : Set} : user_cmd result
+.
 
 Notation "x <- c1 ; c2" := (Bind c1 (fun x => c2)) (right associativity, at level 75).
-Notation "x <<- c1 ; c2" := (BindSymKey c1 (fun x => c2)) (right associativity, at level 75).
-Notation "x <<<- c1 ; c2" := (BindAsymKeys c1 (fun x => c2)) (right associativity, at level 75).
 
-Inductive cmd' : Set -> Type :=
-  (* Plumbing *)
-| Return' {result : Set} (r : result) : cmd' result
-| Bind' {result result' : Set} (c1 : cmd' result') (c2 : result' -> cmd' result) : cmd' result
+Definition queued_messages := fmap user_id (list message).
+Definition user_msg_heap := list (var * message).
 
-| Send' (uid : user_id) (msg : message) : cmd' unit
-| Recv' : cmd' message
-
-| Decrypt' (k : var) (ctxt : message) : cmd' message (* can message be Ciphertext somehow?? *)
-| Encrypt' (k : var) (ptxt : message) : cmd' message
-
-| Sign' (k : var) (msg : message) : cmd' message
-| Verify' (k : option var) (sig : message) : cmd' message
-
-| ProduceHMAC' (k : var) (msg : message) : cmd' message
-| VerifyHMAC' (k : option var) (mac : message) : cmd' message
-
-| GenerateSymKey' (usage : symmetric_usage) : cmd' var
-| GenerateAsymKeys' (usage : asymmetric_usage) : cmd' (var * var)
-
-| Barrier' {result : Set} : cmd' result.
-
-Notation "x <<<<- c1 ; c2" := (Bind' c1 (fun x => c2)) (right associativity, at level 75).
-
-Record user_data :=
-  {uid : user_id ;
+Record user_data : Type := mkUserData {
+   uid      : user_id ;
    key_heap : fmap var key ;
-   msg_heap : fmap var message ;
-   protocol : user_cmd ; 
+   msg_heap : user_msg_heap ;
+   protocol : user_cmd message ; (* todo tbraje: this is wrong, how do we properly handle polymorpic protols?? *)
    is_admin : bool }.
-
-Record user_data' :=
-  {uid' : user_id ;
-   key_heap' : fmap var key ;
-   msg_heap' : fmap var message ;
-   protocol' : forall a : Set, cmd' a ; 
-   is_admin' : bool }.
-
 
 (* The network stores message buffers for each user. Any messages sent to a user are stored here until
    the user calls Recv, at which point they are removed from the buffer and added to the user's msg_heap *)
-Record network := construct_network
-  { users_msg_buffer : fmap user_id (list message) ;
-    trace : list (user_id * message) }.
+Record network := mkNetwork {
+    users_msg_buffer : queued_messages ;
+    trace            : list (user_id * message)
+}.
 
 (* The universe consists of some number of users and a network.
    The key_counter is a temporary hack to keep track of key_ids and make sure two users don't generate
    keys with the same id. *)
-Record universe := construct_universe
-  { users : fmap user_id user_data ;
-    net : network ;
-    key_counter : nat }.
+Record universe := mkUniverse {
+    users       : fmap user_id user_data ;
+    net         : network ;
+    key_counter : nat
+}.
 
 (* Return : net *)
-Definition send_message (msg_var : var) (from_user to_user : user_id) (U : universe) :=
-match U.(users) $? from_user with
-| Some u_data =>
-  match u_data.(msg_heap) $? msg_var with
-  | Some msg =>
-    match (U.(net)).(users_msg_buffer) $? to_user with
-    | Some msg_lst => {| users_msg_buffer := (U.(net)).(users_msg_buffer) $+
-                                             (to_user, msg_lst ++ [msg]) ;
-                         trace := (to_user , msg) :: (U.(net)).(trace) |}
-    | None => U.(net)
-    end
-  | _ => U.(net) (* There was no matching msg to the var *)
-  end
-| _ => U.(net) (* The sender is not valid *)
-end.
+(* Definition send_message (msg_var : var) (from_user to_user : user_id) (U : universe) := *)
+(* match U.(users) $? from_user with *)
+(* | Some u_data => *)
+(*   match u_data.(msg_heap) $? msg_var with *)
+(*   | Some msg => *)
+(*     match (U.(net)).(users_msg_buffer) $? to_user with *)
+(*     | Some msg_lst => {| users_msg_buffer := (U.(net)).(users_msg_buffer) $+ *)
+(*                                              (to_user, msg_lst ++ [msg]) ; *)
+(*                          trace := (to_user , msg) :: (U.(net)).(trace) |} *)
+(*     | None => U.(net) *)
+(*     end *)
+(*   | _ => U.(net) (* There was no matching msg to the var *) *)
+(*   end *)
+(* | _ => U.(net) (* The sender is not valid *) *)
+(* end. *)
 
 (* Return : key_heap *)
-Definition generate_symmetric_key (generating_user : user_id) (key_var : var) (U : universe) (usage : symmetric_usage) :=
-match U.(users) $? generating_user with
-| Some u_data => u_data.(key_heap) $+
-                 (key_var, SymKey {| sym_key_id := U.(key_counter) ;
-                                     sym_generating_user_id := generating_user ;
-                                     sym_usage := usage |})
-| None => $0
-end.
+(* Definition generate_symmetric_key (generating_user : user_id) (key_var : var) (U : universe) (usage : symmetric_usage) := *)
+(* match U.(users) $? generating_user with *)
+(* | Some u_data => u_data.(key_heap) $+ *)
+(*                  (key_var, SymKey {| sym_key_id := U.(key_counter) ; *)
+(*                                      sym_generating_user_id := generating_user ; *)
+(*                                      sym_usage := usage |}) *)
+(* | None => $0 *)
+(* end. *)
 
 (* Return : key_heap *)
-Definition generate_asymmetric_key (generating_user : user_id) (key_var1 key_var2 : var) (U : universe) (usage : asymmetric_usage) :=
-let usage' := match usage with
-              | RSA_Enc => RSA_Dec
-              | RSA_Dec => RSA_Enc
-              | ECDSA_Sig => ECDSA_Ver
-              | ECDSA_Ver => ECDSA_Sig
-              end in
-match U.(users) $? generating_user with
-| Some u_data => u_data.(key_heap) $+
-                 (key_var1, AsymKey {| asym_key_id := U.(key_counter) ;
-                                       asym_generating_user_id := generating_user ;
-                                       asym_usage := usage ;
-                                       asym_paired_key_id := U.(key_counter) + 1 |}) $+
-                 (key_var2, AsymKey {| asym_key_id := U.(key_counter) + 1 ;
-                                       asym_generating_user_id := generating_user ;
-                                       asym_usage := usage' ;
-                                       asym_paired_key_id := U.(key_counter) |})
-| None => $0
-end.
+(* Definition generate_asymmetric_key (generating_user : user_id) (key_var1 key_var2 : var) (U : universe) (usage : asymmetric_usage) := *)
+(* let usage' := match usage with *)
+(*               | RSA_Enc => RSA_Dec *)
+(*               | RSA_Dec => RSA_Enc *)
+(*               | ECDSA_Sig => ECDSA_Ver *)
+(*               | ECDSA_Ver => ECDSA_Sig *)
+(*               end in *)
+(* match U.(users) $? generating_user with *)
+(* | Some u_data => u_data.(key_heap) $+ *)
+(*                  (key_var1, AsymKey {| asym_key_id := U.(key_counter) ; *)
+(*                                        asym_generating_user_id := generating_user ; *)
+(*                                        asym_usage := usage ; *)
+(*                                        asym_paired_key_id := U.(key_counter) + 1 |}) $+ *)
+(*                  (key_var2, AsymKey {| asym_key_id := U.(key_counter) + 1 ; *)
+(*                                        asym_generating_user_id := generating_user ; *)
+(*                                        asym_usage := usage' ; *)
+(*                                        asym_paired_key_id := U.(key_counter) |}) *)
+(* | None => $0 *)
+(* end. *)
 
 (* Return : Universe *)
-Definition recv_message (recving_user : user_id) (U : universe) (x : var) :=
-match (U.(net)).(users_msg_buffer) $? recving_user with
-| Some msg_lst =>
-  match msg_lst with
-  | [] => U
-  | h::t =>
-    match U.(users) $? recving_user with
-    | Some u_data =>
-      match h with
-      | Key_Message sending_user k => 
-        match (U.(users) $? sending_user) with
-        | Some u_data' =>
-          match u_data'.(key_heap) $? k with
-          | Some key =>
-            {| users := U.(users) $+
-                        (recving_user , {| uid := u_data.(uid) ;
-                                           key_heap := u_data.(key_heap) $+ (x, key) ;
-                                           msg_heap := u_data.(msg_heap) ;
-                                           protocol := u_data.(protocol) ;
-                                           is_admin := u_data.(is_admin) |}) ;
-               net := {| users_msg_buffer := (U.(net)).(users_msg_buffer) $+ (recving_user, t) ;
-                         trace := (U.(net)).(trace) |} ;
-               key_counter := U.(key_counter) |}
-          | None => U
-          end
-        | None => U
-        end
-      | _ => {| users := U.(users) $+ 
-                         (recving_user , {| uid := u_data.(uid) ;
-                                            key_heap := u_data.(key_heap) ;
-                                            msg_heap := u_data.(msg_heap) $+ (x, h) ;
-                                            protocol := u_data.(protocol) ;
-                                            is_admin := u_data.(is_admin) |}) ;
-                net := {| users_msg_buffer := (U.(net)).(users_msg_buffer) $+ (recving_user, t) ;
-                trace := (U.(net)).(trace) |} ;
-                key_counter := U.(key_counter) |}
-      end
-    | None => U
-    end
-  end
-| None => U
-end.
+(* Definition recv_message (recving_user : user_id) (U : universe) (x : var) := *)
+(* match (U.(net)).(users_msg_buffer) $? recving_user with *)
+(* | Some msg_lst => *)
+(*   match msg_lst with *)
+(*   | [] => U *)
+(*   | h::t => *)
+(*     match U.(users) $? recving_user with *)
+(*     | Some u_data => *)
+(*       match h with *)
+(*       | Key_Message sending_user k =>  *)
+(*         match (U.(users) $? sending_user) with *)
+(*         | Some u_data' => *)
+(*           match u_data'.(key_heap) $? k with *)
+(*           | Some key => *)
+(*             {| users := U.(users) $+ *)
+(*                         (recving_user , {| uid := u_data.(uid) ; *)
+(*                                            key_heap := u_data.(key_heap) $+ (x, key) ; *)
+(*                                            msg_heap := u_data.(msg_heap) ; *)
+(*                                            protocol := u_data.(protocol) ; *)
+(*                                            is_admin := u_data.(is_admin) |}) ; *)
+(*                net := {| users_msg_buffer := (U.(net)).(users_msg_buffer) $+ (recving_user, t) ; *)
+(*                          trace := (U.(net)).(trace) |} ; *)
+(*                key_counter := U.(key_counter) |} *)
+(*           | None => U *)
+(*           end *)
+(*         | None => U *)
+(*         end *)
+(*       | _ => {| users := U.(users) $+  *)
+(*                          (recving_user , {| uid := u_data.(uid) ; *)
+(*                                             key_heap := u_data.(key_heap) ; *)
+(*                                             msg_heap := u_data.(msg_heap) $+ (x, h) ; *)
+(*                                             protocol := u_data.(protocol) ; *)
+(*                                             is_admin := u_data.(is_admin) |}) ; *)
+(*                 net := {| users_msg_buffer := (U.(net)).(users_msg_buffer) $+ (recving_user, t) ; *)
+(*                 trace := (U.(net)).(trace) |} ; *)
+(*                 key_counter := U.(key_counter) |} *)
+(*       end *)
+(*     | None => U *)
+(*     end *)
+(*   end *)
+(* | None => U *)
+(* end. *)
 
 (* Return : Universe *)
-Definition decrypt_message (u_id : user_id) (msg_var msg_var': var) (U : universe) (key_var : var) :=
-match U.(users) $? u_id with
-| Some u_data =>
-  match u_data.(msg_heap) $? msg_var with
-  | Some msg =>
-    match u_data.(key_heap) $? key_var with
-    | Some (SymKey k) =>
-      match msg with
-      | Ciphertext sending_user msg' k' =>
-        match k.(sym_key_id) with
-        | k' =>
-          match msg' with
-          | Key_Message sending_user km => 
-            match U.(users) $? sending_user with
-            | Some u_data' => 
-              match u_data'.(key_heap) $? km with
-              | Some key => {| users := U.(users) $+
-                                        (u_id , {| uid := u_id ;
-                                                   key_heap := u_data.(key_heap) $+ (msg_var', key) ;
-                                                   msg_heap := u_data.(msg_heap) ;
-                                                   protocol := u_data.(protocol) ;
-                                                   is_admin := u_data.(is_admin) |}) ;
-                               net := U.(net) ;
-                               key_counter := U.(key_counter) |}
-              | None => U
-              end
-           | None => U
-           end
-          | _ => {| users := U.(users) $+
-                             (u_id , {| uid := u_id ;
-                                        key_heap := u_data.(key_heap) ;
-                                        msg_heap := u_data.(msg_heap) $+ (msg_var', msg') ;
-                                        protocol := u_data.(protocol) ;
-                                        is_admin := u_data.(is_admin) |}) ;
-                    net := U.(net) ;
-                    key_counter := U.(key_counter) |}
-          end
-        end
-      | _ => U (* There was nothing to decrypt *)
-      end
-    | Some (AsymKey k) =>
-      match msg with
-      | Ciphertext sending_user msg' k' =>
-        match k.(asym_key_id) with
-        | k' =>
-          match msg' with
-          | Key_Message sending_user km =>
-            match U.(users) $? sending_user with
-            | Some u_data' => 
-              match u_data'.(key_heap) $? km with
-              | Some key => {| users := U.(users) $+
-                                        (u_id , {| uid := u_id ;
-                                                   key_heap := u_data.(key_heap) $+ (msg_var', key) ;
-                                                   msg_heap := u_data.(msg_heap) ;
-                                                   protocol := u_data.(protocol) ;
-                                                   is_admin := u_data.(is_admin) |}) ;
-                               net := U.(net) ;
-                               key_counter := U.(key_counter) |}
-              | None => U
-              end
-           | None => U
-           end
-          | _ => {| users := U.(users) $+
-                             (u_id , {| uid := u_id ;
-                                        key_heap := u_data.(key_heap) ;
-                                        msg_heap := u_data.(msg_heap) $+ (msg_var', msg') ;
-                                        protocol := u_data.(protocol) ;
-                                        is_admin := u_data.(is_admin) |}) ;
-                    net := U.(net) ;
-                    key_counter := U.(key_counter) |}
-          end
-        end
-      | _ => U (* There was nothing to decrypt *)
-      end
-    | _ => U (* Key_var does not correspond to a key *)
-    end
-  | None => U
-  end
-| None => U
-end.
+(* Definition decrypt_message (u_id : user_id) (msg_var msg_var': var) (U : universe) (key_var : var) := *)
+(* match U.(users) $? u_id with *)
+(* | Some u_data => *)
+(*   match u_data.(msg_heap) $? msg_var with *)
+(*   | Some msg => *)
+(*     match u_data.(key_heap) $? key_var with *)
+(*     | Some (SymKey k) => *)
+(*       match msg with *)
+(*       | Ciphertext sending_user msg' k' => *)
+(*         match k.(sym_key_id) with *)
+(*         | k' => *)
+(*           match msg' with *)
+(*           | Key_Message sending_user km =>  *)
+(*             match U.(users) $? sending_user with *)
+(*             | Some u_data' =>  *)
+(*               match u_data'.(key_heap) $? km with *)
+(*               | Some key => {| users := U.(users) $+ *)
+(*                                         (u_id , {| uid := u_id ; *)
+(*                                                    key_heap := u_data.(key_heap) $+ (msg_var', key) ; *)
+(*                                                    msg_heap := u_data.(msg_heap) ; *)
+(*                                                    protocol := u_data.(protocol) ; *)
+(*                                                    is_admin := u_data.(is_admin) |}) ; *)
+(*                                net := U.(net) ; *)
+(*                                key_counter := U.(key_counter) |} *)
+(*               | None => U *)
+(*               end *)
+(*            | None => U *)
+(*            end *)
+(*           | _ => {| users := U.(users) $+ *)
+(*                              (u_id , {| uid := u_id ; *)
+(*                                         key_heap := u_data.(key_heap) ; *)
+(*                                         msg_heap := u_data.(msg_heap) $+ (msg_var', msg') ; *)
+(*                                         protocol := u_data.(protocol) ; *)
+(*                                         is_admin := u_data.(is_admin) |}) ; *)
+(*                     net := U.(net) ; *)
+(*                     key_counter := U.(key_counter) |} *)
+(*           end *)
+(*         end *)
+(*       | _ => U (* There was nothing to decrypt *) *)
+(*       end *)
+(*     | Some (AsymKey k) => *)
+(*       match msg with *)
+(*       | Ciphertext sending_user msg' k' => *)
+(*         match k.(asym_key_id) with *)
+(*         | k' => *)
+(*           match msg' with *)
+(*           | Key_Message sending_user km => *)
+(*             match U.(users) $? sending_user with *)
+(*             | Some u_data' =>  *)
+(*               match u_data'.(key_heap) $? km with *)
+(*               | Some key => {| users := U.(users) $+ *)
+(*                                         (u_id , {| uid := u_id ; *)
+(*                                                    key_heap := u_data.(key_heap) $+ (msg_var', key) ; *)
+(*                                                    msg_heap := u_data.(msg_heap) ; *)
+(*                                                    protocol := u_data.(protocol) ; *)
+(*                                                    is_admin := u_data.(is_admin) |}) ; *)
+(*                                net := U.(net) ; *)
+(*                                key_counter := U.(key_counter) |} *)
+(*               | None => U *)
+(*               end *)
+(*            | None => U *)
+(*            end *)
+(*           | _ => {| users := U.(users) $+ *)
+(*                              (u_id , {| uid := u_id ; *)
+(*                                         key_heap := u_data.(key_heap) ; *)
+(*                                         msg_heap := u_data.(msg_heap) $+ (msg_var', msg') ; *)
+(*                                         protocol := u_data.(protocol) ; *)
+(*                                         is_admin := u_data.(is_admin) |}) ; *)
+(*                     net := U.(net) ; *)
+(*                     key_counter := U.(key_counter) |} *)
+(*           end *)
+(*         end *)
+(*       | _ => U (* There was nothing to decrypt *) *)
+(*       end *)
+(*     | _ => U (* Key_var does not correspond to a key *) *)
+(*     end *)
+(*   | None => U *)
+(*   end *)
+(* | None => U *)
+(* end. *)
 
 (* Return : msg_heap *)
-Definition encrypt_message (u_id : user_id) (msg_var msg_var': var) (key_var : var) (U : universe) :=
-match U.(users) $? u_id with
-| Some u_data => 
-  match u_data.(msg_heap) $? msg_var with
-  | Some msg => 
-    match u_data.(key_heap) $? key_var with
-    | Some (AsymKey k) => 
-      match k.(asym_usage) with
-      | RSA_Enc => u_data.(msg_heap) $+ 
-                   (msg_var', (Ciphertext u_id msg k.(asym_paired_key_id)))
-      | _ => u_data.(msg_heap)
-      end
-    | Some (SymKey k') =>
-      match k'.(sym_usage) with
-      | HMAC => u_data.(msg_heap)
-      | _ => u_data.(msg_heap) $+
-             (msg_var', (Ciphertext u_id msg k'.(sym_key_id)))
-      end
-    | _ => u_data.(msg_heap)
-    end
-  | None => u_data.(msg_heap)
-  end
-| None => $0
-end.
+(* Definition encrypt_message (u_id : user_id) (msg_var msg_var': var) (key_var : var) (U : universe) := *)
+(* match U.(users) $? u_id with *)
+(* | Some u_data =>  *)
+(*   match u_data.(msg_heap) $? msg_var with *)
+(*   | Some msg =>  *)
+(*     match u_data.(key_heap) $? key_var with *)
+(*     | Some (AsymKey k) =>  *)
+(*       match k.(asym_usage) with *)
+(*       | RSA_Enc => u_data.(msg_heap) $+  *)
+(*                    (msg_var', (Ciphertext u_id msg k.(asym_paired_key_id))) *)
+(*       | _ => u_data.(msg_heap) *)
+(*       end *)
+(*     | Some (SymKey k') => *)
+(*       match k'.(sym_usage) with *)
+(*       | HMAC => u_data.(msg_heap) *)
+(*       | _ => u_data.(msg_heap) $+ *)
+(*              (msg_var', (Ciphertext u_id msg k'.(sym_key_id))) *)
+(*       end *)
+(*     | _ => u_data.(msg_heap) *)
+(*     end *)
+(*   | None => u_data.(msg_heap) *)
+(*   end *)
+(* | None => $0 *)
+(* end. *)
 
 (* Return : msg_heap *)
-Definition sign (signer : user_id) (key_var msg_var signed_msg_var : var) (U : universe) :=
-match U.(users) $? signer with
-| Some u_data =>
-  match u_data.(msg_heap) $? msg_var with
-  | Some msg =>
-    match u_data.(key_heap) $? key_var with
-    | Some (AsymKey k) =>
-      match k.(asym_usage) with
-      | ECDSA_Sig => u_data.(msg_heap) $+
-                     (signed_msg_var, (Signature k.(asym_paired_key_id) signer msg))
-      | _ => u_data.(msg_heap)
-      end
-    | _ => u_data.(msg_heap)
-    end
-  | None => u_data.(msg_heap)
-  end
-| None => $0
-end.
+(* Definition sign (signer : user_id) (key_var msg_var signed_msg_var : var) (U : universe) := *)
+(* match U.(users) $? signer with *)
+(* | Some u_data => *)
+(*   match u_data.(msg_heap) $? msg_var with *)
+(*   | Some msg => *)
+(*     match u_data.(key_heap) $? key_var with *)
+(*     | Some (AsymKey k) => *)
+(*       match k.(asym_usage) with *)
+(*       | ECDSA_Sig => u_data.(msg_heap) $+ *)
+(*                      (signed_msg_var, (Signature k.(asym_paired_key_id) signer msg)) *)
+(*       | _ => u_data.(msg_heap) *)
+(*       end *)
+(*     | _ => u_data.(msg_heap) *)
+(*     end *)
+(*   | None => u_data.(msg_heap) *)
+(*   end *)
+(* | None => $0 *)
+(* end. *)
 
 (* Return : msg_heap *)
-Definition produceHMAC (producer : user_id) (key_var msg_var HMAC_var : var) (U : universe) :=
-match U.(users) $? producer with
-| Some u_data => 
-  match u_data.(msg_heap) $? msg_var with
-  | Some msg => 
-    match u_data.(key_heap) $? key_var with
-    | Some (SymKey k) =>
-      match k.(sym_usage) with
-      | HMAC => u_data.(msg_heap) $+
-                (HMAC_var, (HMAC_Message producer k.(sym_key_id) msg))
-      | _ => u_data.(msg_heap)
-      end
-    | _ => u_data.(msg_heap)
-    end
-  | None => u_data.(msg_heap)
-  end
-| None => $0
-end.
+(* Definition produceHMAC (producer : user_id) (key_var msg_var HMAC_var : var) (U : universe) := *)
+(* match U.(users) $? producer with *)
+(* | Some u_data =>  *)
+(*   match u_data.(msg_heap) $? msg_var with *)
+(*   | Some msg =>  *)
+(*     match u_data.(key_heap) $? key_var with *)
+(*     | Some (SymKey k) => *)
+(*       match k.(sym_usage) with *)
+(*       | HMAC => u_data.(msg_heap) $+ *)
+(*                 (HMAC_var, (HMAC_Message producer k.(sym_key_id) msg)) *)
+(*       | _ => u_data.(msg_heap) *)
+(*       end *)
+(*     | _ => u_data.(msg_heap) *)
+(*     end *)
+(*   | None => u_data.(msg_heap) *)
+(*   end *)
+(* | None => $0 *)
+(* end. *)
 
 (* Return : Universe *)
-Definition verify (verifier : user_id) (key_var signed_msg_var verified_msg_var : var) (U : universe) :=
-match U.(users) $? verifier with
-| Some u_data =>
-  match u_data.(msg_heap) $? signed_msg_var with
-  | Some sym_msg =>
-    match u_data.(key_heap) $? key_var with
-    | Some (AsymKey k) =>
-      match sym_msg with
-      | Signature k_id signer msg =>
-        if k_id =? k.(asym_paired_key_id)
-        then match msg with
-             | Key_Message signer key_v => 
-               match U.(users) $? signer with
-               | Some u_data' => 
-                 match u_data'.(key_heap) $? key_v with
-                 | Some key => {| users := U.(users) $+
-                                           (verifier, {| uid := verifier ;
-                                                         key_heap := u_data.(key_heap) $+
-                                                                     (verified_msg_var, key) ;
-                                                         msg_heap := u_data.(msg_heap) ;
-                                                         protocol := u_data.(protocol) ;
-                                                         is_admin := u_data.(is_admin) |}) ;
-                                  net := U.(net) ;
-                                  key_counter := U.(key_counter) |}
-                 | None => U
-                 end
-               | None => U
-               end
-             | _ => {| users := U.(users) $+
-                                (verifier, {| uid := verifier ;
-                                              key_heap := u_data.(key_heap) ;
-                                              msg_heap := u_data.(msg_heap) $+
-                                                          (verified_msg_var, msg) ;
-                                              protocol := u_data.(protocol) ;
-                                              is_admin := u_data.(is_admin) |}) ;
-                       net := U.(net) ;
-                       key_counter := U.(key_counter) |}
-             end
-        else U
-      | _ => U
-      end
-    | _ => U
-    end
-  | None => U
-  end
-| None => U
-end.
+(* Definition verify (verifier : user_id) (key_var signed_msg_var verified_msg_var : var) (U : universe) := *)
+(* match U.(users) $? verifier with *)
+(* | Some u_data => *)
+(*   match u_data.(msg_heap) $? signed_msg_var with *)
+(*   | Some sym_msg => *)
+(*     match u_data.(key_heap) $? key_var with *)
+(*     | Some (AsymKey k) => *)
+(*       match sym_msg with *)
+(*       | Signature k_id signer msg => *)
+(*         if k_id =? k.(asym_paired_key_id) *)
+(*         then match msg with *)
+(*              | Key_Message signer key_v =>  *)
+(*                match U.(users) $? signer with *)
+(*                | Some u_data' =>  *)
+(*                  match u_data'.(key_heap) $? key_v with *)
+(*                  | Some key => {| users := U.(users) $+ *)
+(*                                            (verifier, {| uid := verifier ; *)
+(*                                                          key_heap := u_data.(key_heap) $+ *)
+(*                                                                      (verified_msg_var, key) ; *)
+(*                                                          msg_heap := u_data.(msg_heap) ; *)
+(*                                                          protocol := u_data.(protocol) ; *)
+(*                                                          is_admin := u_data.(is_admin) |}) ; *)
+(*                                   net := U.(net) ; *)
+(*                                   key_counter := U.(key_counter) |} *)
+(*                  | None => U *)
+(*                  end *)
+(*                | None => U *)
+(*                end *)
+(*              | _ => {| users := U.(users) $+ *)
+(*                                 (verifier, {| uid := verifier ; *)
+(*                                               key_heap := u_data.(key_heap) ; *)
+(*                                               msg_heap := u_data.(msg_heap) $+ *)
+(*                                                           (verified_msg_var, msg) ; *)
+(*                                               protocol := u_data.(protocol) ; *)
+(*                                               is_admin := u_data.(is_admin) |}) ; *)
+(*                        net := U.(net) ; *)
+(*                        key_counter := U.(key_counter) |} *)
+(*              end *)
+(*         else U *)
+(*       | _ => U *)
+(*       end *)
+(*     | _ => U *)
+(*     end *)
+(*   | None => U *)
+(*   end *)
+(* | None => U *)
+(* end. *)
 
 (* Return : Universe *)
-Definition verifyHMAC (verifier : user_id) (key_var HMAC_var verified_msg_var : var) (U : universe) :=
-match U.(users) $? verifier with
-| Some u_data => 
-  match u_data.(msg_heap) $? HMAC_var with
-  | Some HMAC_msg => 
-    match u_data.(key_heap) $? key_var with
-    | Some (SymKey k) => 
-      match HMAC_msg with
-      | HMAC_Message sender k_id msg => 
-        if k_id =? k.(sym_key_id)
-        then match msg with
-             | Key_Message sender' key_var' => 
-               match U.(users) $? sender with 
-               | Some u_data' => 
-                 match u_data'.(key_heap) $? key_var' with
-                 | Some key => {| users := U.(users) $+
-                                           (verifier, {| uid := verifier ;
-                                                         key_heap := u_data.(key_heap) $+ 
-                                                                     (verified_msg_var, key) ;
-                                                         msg_heap := u_data.(msg_heap) ;
-                                                         protocol := u_data.(protocol) ;
-                                                         is_admin := u_data.(is_admin) |}) ;
-                                   net := U.(net) ;
-                                   key_counter := U.(key_counter) |}
-                 | None => U
-                 end
-               | None => U
-               end
-             | _ => {| users := U.(users) $+
-                                (verifier, {| uid := verifier ;
-                                              key_heap := u_data.(key_heap) ;
-                                              msg_heap := u_data.(msg_heap) $+
-                                                          (verified_msg_var, msg) ;
-                                              protocol := u_data.(protocol) ;
-                                              is_admin := u_data.(is_admin) |}) ;
-                       net := U.(net) ;
-                       key_counter := U.(key_counter) |}
-             end
-        else U
-      | _ => U
-      end
-    | _ => U
-    end
-  | None => U
-  end
-| None => U
-end.
+(* Definition verifyHMAC (verifier : user_id) (key_var HMAC_var verified_msg_var : var) (U : universe) := *)
+(* match U.(users) $? verifier with *)
+(* | Some u_data =>  *)
+(*   match u_data.(msg_heap) $? HMAC_var with *)
+(*   | Some HMAC_msg =>  *)
+(*     match u_data.(key_heap) $? key_var with *)
+(*     | Some (SymKey k) =>  *)
+(*       match HMAC_msg with *)
+(*       | HMAC_Message sender k_id msg =>  *)
+(*         if k_id =? k.(sym_key_id) *)
+(*         then match msg with *)
+(*              | Key_Message sender' key_var' =>  *)
+(*                match U.(users) $? sender with  *)
+(*                | Some u_data' =>  *)
+(*                  match u_data'.(key_heap) $? key_var' with *)
+(*                  | Some key => {| users := U.(users) $+ *)
+(*                                            (verifier, {| uid := verifier ; *)
+(*                                                          key_heap := u_data.(key_heap) $+  *)
+(*                                                                      (verified_msg_var, key) ; *)
+(*                                                          msg_heap := u_data.(msg_heap) ; *)
+(*                                                          protocol := u_data.(protocol) ; *)
+(*                                                          is_admin := u_data.(is_admin) |}) ; *)
+(*                                    net := U.(net) ; *)
+(*                                    key_counter := U.(key_counter) |} *)
+(*                  | None => U *)
+(*                  end *)
+(*                | None => U *)
+(*                end *)
+(*              | _ => {| users := U.(users) $+ *)
+(*                                 (verifier, {| uid := verifier ; *)
+(*                                               key_heap := u_data.(key_heap) ; *)
+(*                                               msg_heap := u_data.(msg_heap) $+ *)
+(*                                                           (verified_msg_var, msg) ; *)
+(*                                               protocol := u_data.(protocol) ; *)
+(*                                               is_admin := u_data.(is_admin) |}) ; *)
+(*                        net := U.(net) ; *)
+(*                        key_counter := U.(key_counter) |} *)
+(*              end *)
+(*         else U *)
+(*       | _ => U *)
+(*       end *)
+(*     | _ => U *)
+(*     end *)
+(*   | None => U *)
+(*   end *)
+(* | None => U *)
+(* end. *)
 
 
 (* Ping Protocol *)
 
 (* U.(users) 
    Check on both ends that received message == "Hello" *)
+
+Example pingUser1 : user_id -> user_cmd message := fun uid =>
+  a <- GenerateAsymKeys RSA_Enc ;
+  b <- Send uid (Key_Message 0 (fst a)) ;
+  c <- GenerateAsymKeys ECDSA_Sig ;
+  d <- Send uid (Key_Message 0 (fst c)) ;
+  e <- Sign (snd c) (Plaintext 0 "Hello") ;
+  f <- Encrypt (snd a) e ;
+  g <- Send uid f ;
+  Recv. (* Had better be Plaintext 1 "Hello" *)
+
+Example pingUser2 : user_id -> user_cmd message := fun uid =>
+  a <- Recv ;
+  b <- Recv ;
+  c <- Recv ;
+  (* d <- Decrypt a c; *)
+  (* e <- Verify (match b with *)
+  (*                  | Key_Message 0 k => Some k *)
+  (*                  | _ => None *)
+  (*                  end) d ; *)
+  (* _ <- Send uid e *)
+  Return a. (* delete me *)
+  (* Return e. (* Had better be Plaintext "Hello" *) *)
+
 Example ping_users :=
  $0 $+ (0, {| uid := 0 ;
               key_heap := $0 ;
-              msg_heap := $0 ;
-              protocol := a <<<- GenerateAsymKeys RSA_Enc ;
-                          b <-   Send 1 (Key_Message 0 (fst a)) ;
-                          c <<<- GenerateAsymKeys ECDSA_Sig ;
-                          d <- Send 1 (Key_Message 0 (fst c)) ;
-                          e <- Sign (snd c) (Plaintext 0 "Hello") ;
-                          f <- Encrypt (snd a) e ;
-                          g <- Send 1 f ;
-                          Recv ;
+              msg_heap := nil ;
+              protocol := pingUser1 1 ;
               is_admin := false |})
     $+ (1 , {| uid := 1 ;
                key_heap := $0 ;
-               msg_heap := $0 ;
-               protocol := a <- Recv ;
-                           b <- Recv ;
-                           c <- Recv ;
-                           d <- Decrypt (match a with
-                                           | Key_Message 0 k' => Some k'
-                                           | _ => None
-                                           end) c ;
-                           e <- Verify (match b with
-                                          | Key_Message 0 k => Some k
-                                          | _ => None
-                                          end) d ;
-                           Send 0 e ;
-is_admin := false |}).
-
-
-Example pingUser1 :=
-  a <<<<- GenerateAsymKeys' RSA_Enc ;
-  b <<<<- Send' 1 (Key_Message 0 (fst a)) ;
-  c <<<<- GenerateAsymKeys' ECDSA_Sig ;
-  d <<<<- Send' 1 (Key_Message 0 (fst c)) ;
-  e <<<<- Sign' (snd c) (Plaintext 0 "Hello") ;
-  f <<<<- Encrypt' (snd a) e ;
-  g <<<<- Send' 1 f ;
-  Recv'.
-
-Example pingUser2 :=
-  a <<<<- Recv' ;
-  b <<<<- Recv' ;
-  c <<<<- Recv' ;
-  d <<<<- Decrypt' (match a with
-                    | Key_Message 0 k' => Some k'
-                    | _ => None
-                    end) c;
-  e <<<<- Verify' (match b with
-                   | Key_Message 0 k => Some k
-                   | _ => None
-                   end) d ;
-  Send' 0 e.
-
-(* Example ping_users' := *)
-(*  $0 $+ (0, {| uid' := 0 ; *)
-(*               key_heap' := $0 ; *)
-(*               msg_heap' := $0 ; *)
-(*               protocol' := pingUser1; *)
-(*               is_admin' := false |}). *)
-(*     $+ (1 , {| uid := 1 ; *)
-(*                key_heap := $0 ; *)
-(*                msg_heap := $0 ; *)
-(*                protocol := pingUser2; *)
-(*                is_admin := false |}). *)
-
-
+               msg_heap := nil ;
+               protocol := pingUser2 0 ;
+               is_admin := false |}).
 
 (* Ping Universe *)
 Example ping_universe :=
@@ -554,6 +521,44 @@ Example ping_universe :=
    net := {| users_msg_buffer := $0 $+ (0, []) $+ (1, []) ;
              trace := [] |} ;
    key_counter := 0 |}.
+
+
+
+Inductive step_user : forall A, queued_messages * user_msg_heap * user_cmd A -> queued_messages * user_msg_heap * user_cmd A -> Prop :=
+  (* Plumbing *)
+| StepBindRecur : forall result result' q q' h h' (cmd1 cmd1' : user_cmd result) (cmd2 : result -> user_cmd result'),
+    step_user (q, h, cmd1) (q', h', cmd1')
+    -> step_user (q, h, Bind cmd1 cmd2) (q', h', Bind cmd1' cmd2)
+| StepBindProceed : forall (result result' : Set) q h (v : result') (cmd : result' -> user_cmd result),
+    step_user (q, h, Bind (Return v) cmd) (q, h, cmd v)
+
+(* Comms *)
+(* | Send (uid : user_id) (msg : message) : user_cmd unit *)
+(* | Recv : user_cmd message *)
+| StepRecv : forall uid q h msg msgs,
+    q $? uid = Some (cons msg msgs) (* we have a message waiting for us! *)
+    -> step_user (q, h, Recv) (q, h, Return msg)
+| StepSend : forall q h uid msg,
+    step_user (q, h, Send uid msg) (q, h, Return tt)
+
+(* Crypto! *)
+
+(* | Decrypt (k : var) (ctxt : message) : user_cmd message (* can message be Ciphertext somehow?? *) *)
+(* | Encrypt (k : var) (ptxt : message) : user_cmd message *)
+
+(* | Sign (k : var) (msg : message) : user_cmd message *)
+(* | Verify (k : option var) (sig : message) : user_cmd message *)
+
+(* | ProduceHMAC (k : var) (msg : message) : user_cmd message *)
+(* | VerifyHMAC (k : option var) (mac : message) : user_cmd message *)
+
+(* | GenerateSymKey (usage : symmetric_usage) : user_cmd var *)
+(* | GenerateAsymKeys (usage : asymmetric_usage) : user_cmd (var * var) *)
+ 
+(* | Barrier {result : Set} : user_cmd result. *)
+.
+
+
 
 Inductive step : universe -> universe -> Prop :=
 | StepSign : forall signer key_var msg_var signed_msg_var U u_data k msg msg_heap' users' signed_message,
